ironfleet/weekly_summary/week6.md
@@ -1,0 +1,12 @@
+### Last Week
+
+- Complete about half of the impl -> protocol refinement
+
+### Discuss
+
+- About protocol -> spec
+  - Inspired Manos's course: can we use inductive invariants?
+    - Problem: How do we find inductive invariants?
+
+- About the poster?
+  - Just show the methodology of IronFleet?
